compiler/src/compiler/FlattenExpr.v
@@ -14,6 +14,7 @@ Require Import coqutil.Datatypes.PropSet.
 Require Import compiler.Simp.
 Require Import coqutil.Datatypes.String.
 Require Import compiler.FlattenExprDef.
+Require Import compiler.SimplWordExpr.
 
 Open Scope Z_scope.
 
@@ -362,7 +363,7 @@ Section FlattenExpr1.
       eapply @FlatImp.exec.seq.
       + eapply IHe; try eassumption. maps.
       + intros. simpl in *. simp.
-        eapply @FlatImp.exec.load; t_safe; try eassumption. solve_MetricLog.
+        eapply @FlatImp.exec.load; t_safe; rewrite ?add_0_r; try eassumption; solve_MetricLog.
 
     - (* expr.op *)
       eapply seq_with_modVars.
@@ -632,7 +633,7 @@ Section FlattenExpr1.
         eapply @FlatImp.exec.seq.
         * eapply flattenExpr_correct_with_modVars; try eassumption; maps.
         * intros. simpl in *. simp.
-          eapply @FlatImp.exec.store; try eassumption.
+          eapply @FlatImp.exec.store; rewrite ?add_0_r; try eassumption.
           { eapply flattenExpr_valid_resVar in E; maps. }
           { repeat eexists; repeat (split || eassumption || solve_MetricLog); maps. }
 
